\documentclass{article}

\setlength{\headsep}{0.75 in}
\setlength{\parindent}{0 in}
\setlength{\parskip}{0.1 in}

%=====================================================
% Add PACKAGES Here (You typically would not need to):
%=====================================================

\usepackage{xcolor}
\usepackage[margin=1in]{geometry}
\usepackage{amsmath,amsthm}
\usepackage{fancyhdr}
\usepackage{enumitem}
\usepackage{graphicx}
\usepackage{amsmath, amssymb}  % Include the amsmath and amssymb packages for mathematical symbols

%=====================================================
% Ignore This Part (But Do NOT Delete It:)
%=====================================================

\theoremstyle{definition}
\newtheorem{problem}{Problem}
\newtheorem*{fun}{Fun with Algorithms}
\newtheorem*{challenge}{Challenge Yourself}
\def\fline{\rule{0.75\linewidth}{0.5pt}}
\newcommand{\finishline}{\begin{center}\fline\end{center}}
\newtheorem*{solution*}{Solution}
\newenvironment{solution}{\begin{solution*}}{{\finishline} \end{solution*}}
\newcommand{\grade}[1]{\hfill{\textbf{($\mathbf{#1}$ points)}}}
\newcommand{\thisdate}{February 20, 2024}
\newcommand{\thissemester}{\textbf{Rutgers: Spring 2024}}
\newcommand{\thiscourse}{ECE 509: Convex Optimization} 
\newcommand{\thishomework}{Number} 
\newcommand{\thisname}{Name} 
\newcommand{\thisextension}{Yes/No} 

\headheight 40pt              
\headsep 10pt
\renewcommand{\headrulewidth}{0pt}
\pagestyle{fancy}

\newcommand{\thisheading}{
   \noindent
   \begin{center}
   \framebox{
      \vbox{\vspace{2mm}
    \hbox to 6.28in { \textbf{\thiscourse \hfill \thissemester} }
       \vspace{4mm}
       \hbox to 6.28in { {\Large \hfill Homework \#\thishomework \hfill} }
       \vspace{2mm}
         \hbox to 6.28in { { \hfill \thisdate  \hfill} }
       \vspace{2mm}
       \hbox to 6.28in { \emph{Name: \thisname \hfill Extension: \thisextension}}
      \vspace{2mm}}
      }
   \end{center}
   \bigskip
}

%=====================================================
% Some useful MACROS (you can define your own in the same exact way also)
%=====================================================


\newcommand{\ceil}[1]{{\left\lceil{#1}\right\rceil}}
\newcommand{\floor}[1]{{\left\lfloor{#1}\right\rfloor}}
\newcommand{\prob}[1]{\Pr\paren{#1}}
\newcommand{\expect}[1]{\Exp\bracket{#1}}
\newcommand{\var}[1]{\textnormal{Var}\bracket{#1}}
\newcommand{\set}[1]{\ensuremath{\left\{ #1 \right\}}}
\newcommand{\poly}{\mbox{\rm poly}}


%=====================================================
% Fill Out This Part With Your Own Information:
%=====================================================


\renewcommand{\thishomework}{3} %Homework number
\renewcommand{\thisname}{Ravi Raghavan} % Enter your name here
\renewcommand{\thisextension}{No} % Pick only one of the two options accordingly

\begin{document}

\thisheading
\vspace{-0.75cm}


%=====================================================
% LaTeX Tip: You can erase this part from here.... 
%=====================================================		

\finishline

%=====================================================
% LaTeX Tip: ... to here
%=====================================================	


\bigskip

\begin{problem} Suppose $f: \mathbb{R} \rightarrow \mathbb{R}$ is convex, and $a, b \in dom f$ with $a < b$
    \begin{enumerate}
        \item[(a)] Show that 
                    \begin{equation}
                        \label{eq:example}
                            f(x) \leq \frac{b - x}{b - a} f(a) + \frac{x - a}{b - a} f(b)
                    \end{equation}
                    for all $x \in [a, b]$. 

                    \begin{solution}
                        Let us have $\theta \in \mathbb{R}$ where $0 \leq \theta \leq 1$. Since $x \in [a, b]$, we can define $x$ as $\theta a + (1 - \theta)b $ \newline 

                        Based on the definition of a convex function, we know that $f(\theta a + (1 - \theta)b) \leq \theta f(a) + (1 - \theta) f(b)$ \newline 

                        $f(x) \leq \theta f(a) + (1 - \theta) f(b)$ \newline 

                        $x = \theta a + b - \theta b$ \newline 

                        $x - b = \theta (a - b)$ \newline 

                        $\frac{x - b}{a - b} = \frac{b - x}{b - a} = \theta$ \newline 

                        $1 - \theta = 1 - \frac{b - x}{b - a} = \frac{x - a}{b - a}$ \newline 

                        $f(x) \leq \frac{b - x}{b - a} f(a) + \frac{x - a}{b - a} f(b)$ \newline 
                    \end{solution}
        \item[(b)] Show that 
                    \begin{equation}
                        \label{eq:example}
                            \frac{f(x) - f(a)}{x - a} \leq \frac{f(b) - f(a)}{b - a} \leq \frac{f(b) - f(x)}{b - x} 
                    \end{equation}
                    for all $x \in (a, b)$. Draw a sketch that illustrates this inequality

                    \begin{solution}
                        \begin{equation}
                        \label{eq:example}
                            f(x) \leq \frac{b - x}{b - a} f(a) + \frac{x - a}{b - a} f(b)
                    \end{equation}

                    Multiply both sides by $b - a$ \newline 

                    \begin{equation}
                        \label{eq:example}
                            f(x) (b - a) \leq (b - x) f(a) + (x - a) f(b)
                    \end{equation}

                    \begin{equation}
                        \label{eq:example}
                            f(x) (b - a) \leq (b - a) f(a) - (x - a) f(a) + (x - a) f(b)
                    \end{equation}

                    \begin{equation}
                        \label{eq:example}
                            (f(x) - f(a)) (b - a) \leq - (x - a) f(a) + (x - a) f(b)
                    \end{equation}

                    \begin{equation}
                        \label{eq:example}
                            (f(x) - f(a)) (b - a) \leq (x - a) (f(b) - f(a))
                    \end{equation}

                    Divide both sides by $x - a$

                    \begin{equation}
                        \label{eq:example}
                            \frac{(f(x) - f(a))}{x - a} (b - a) \leq (f(b) - f(a))
                    \end{equation}

                    Divide both sides by $b - a$

                    \begin{equation}
                        \label{eq:example}
                            \frac{(f(x) - f(a))}{x - a}  \leq \frac{(f(b) - f(a))}{b - a}
                    \end{equation}

Now, let's start with the same inequality, $f(x) (b - a) \leq (b - x) f(a) + (x - a) f(b)$, and work it in a new direction


                    \begin{equation}
                        \label{eq:example}
                            f(x) (b - a) \leq (b - x) f(a) + (x - a) f(b)
                    \end{equation}

                    \begin{equation}
                        \label{eq:example}
                            f(x) (b - a) \leq (b - x) f(a) + (b - a) f(b) - (b - x) f(b)
                    \end{equation}

                    \begin{equation}
                        \label{eq:example}
                            (f(x) - f(b)) (b - a) \leq (b - x) (f(a) - f(b))
                    \end{equation}

                    \begin{equation}
                        \label{eq:example}
                            (f(b) - f(x)) (b - a) \geq (b - x) (f(b) - f(a))
                    \end{equation}

Multiply each side by $\frac{1}{(b - x)(b - a)}$

                    \begin{equation}
                        \label{eq:example}
                            \frac{f(b) - f(x)}{b - x} \geq \frac{f(b) - f(a)}{b - a}
                    \end{equation}

Put together we get: \newline 

\begin{equation}
                        \label{eq:example}
                            \frac{f(x) - f(a)}{x - a}  \leq \frac{f(b) - f(a)}{b - a} \leq \frac{f(b) - f(x)}{b - x} 
                    \end{equation}

Note: The sketch is on the next page. 
\newpage 
                    \begin{figure}[h!]
        \centering
        \includegraphics[width=\textwidth]{1B.jpg}
        \caption{Sketch of Inequality in (B)}
    \end{figure}  

    Geometrically, this sketch depicts the inequality in Part (B). It shows that the slope of the line connecting points $(a, f(a))$ and $(b, f(b))$ is GREATER than the slope of the line connecting points $(a, f(a))$ and $(x, f(x))$. The sketch also shows that slope of the line connecting points $(a, f(a))$ and $(b, f(b))$ is LESS than the slope of the line connecting points $(x, f(x))$ and $(b, f(b))$
                    
                    \end{solution}
                    
        \item[(c)] Suppose $f$ is differentiable. Use the result in (b) to show that 
        \begin{equation}
                        \label{eq:example}
                            f'(a) \leq  \frac{f(b) - f(a)}{b - a} \leq f'(b)
                    \end{equation}

                \begin{solution}
                    We know that, for a convex function, the first-order Taylor approximation is in fact a global underestimator of the function. Hence, we can say the following: \newline 

                    $f(a) + f'(a) (x - a) \leq f(x)$ \newline 
                    $f'(a) \leq \frac{f(x) - f(a)}{x - a}$ \newline 

                    $f(b) + f'(b) (x - b) \leq f(x)$ \newline 
                    $f'(b) (b - x) \geq f(b) - f(x)$ \newline 
                    $f'(b) \geq \frac{f(b) - f(x)}{b - x}$ \newline
                    $\frac{f(b) - f(x)}{b - x} \leq f'(b)$ \newline


                    We know that $f'(a) \leq \frac{f(x) - f(a)}{x - a}$, $\frac{f(x) - f(a)}{x - a}  \leq \frac{f(b) - f(a)}{b - a} \leq \frac{f(b) - f(x)}{b - x}$, and $\frac{f(b) - f(x)}{b - x} \leq f'(b)$, we can say that: \newline 

                    $f'(a) \leq \frac{f(x) - f(a)}{x - a}  \leq \frac{f(b) - f(a)}{b - a} \leq \frac{f(b) - f(x)}{b - x} \leq f'(b)$ \newline 

                    $f'(a) \leq \frac{f(b) - f(a)}{b - a} \leq  f'(b)$ \newline 
                \end{solution}

        \item[(d)] Suppose $f$ is twice differentiable. Use the result in $(c)$ to show that $f''(a) \geq 0$ and $f''(b) \geq 0$

            \begin{solution}
                The result in Part (c) shows us that $f'(a) \leq  \frac{f(b) - f(a)}{b - a} \leq f'(b)$ \newline 

                From this, since $f'(a) \leq f'(b)$, we can go one step further and say that $\frac{f'(b) - f'(a)}{b - a} \geq 0$ \newline 

                From this, we can take the limit and see that: 

                $f''(a) = \lim_{b\to a} \frac{f'(b) - f'(a)}{b - a} \geq 0$ \newline 

                By extension, we can say that

                $f''(b) = \lim_{a\to b} \frac{f'(b) - f'(a)}{b - a} \geq 0$
                
                
                
            \end{solution}
    \end{enumerate}
\end{problem}

\begin{problem}
    Show that a continuous function $f: \mathbb{R}^n \rightarrow \mathbb{R}$ is convex if and only if for every line segment, its average value on the segment is less than or equal to the average of its values at the endpoints of the segment: For every $x, y \in \mathbb{R}^n$,

    \begin{equation}
        \label{eq:example}
            \int_{0}^{1} f(x + \lambda(y - x)) \,d \lambda \leq \frac{f(x) + f(y)}{2}
    \end{equation}

    \begin{solution}
        Step 1: The "Only If" Part \newline 
        We know that $f$ is convex and that $f$ is continuous. Our goal is to prove that, for every line segment, its average value on the segment is less than or equal to the average of its values at the endpoints of the segment.  \newline 

        Let's re-arrange the insides of the integral to write its mathematical equivalent: \newline 

        \begin{equation}
        \label{eq:example}
            \int_{0}^{1} f((1 - \lambda)x + \lambda y) \,d \lambda
    \end{equation}

Based on the definition of convexity, we know that $f((1 - \lambda)x + \lambda y) \leq \lambda f(y) + (1 - \lambda) f(x)$
    \begin{equation}
        \label{eq:example}
            \int_{0}^{1} f((1 - \lambda)x + \lambda y) \,d \lambda \leq \int_{0}^{1} \lambda f(y) + (1 - \lambda) f(x) \,d \lambda
    \end{equation}

Let's evaluate this integral \newline 
\begin{equation}
        \label{eq:example}
            \int_{0}^{1} \lambda f(y) + (1 - \lambda) f(x) \,d \lambda =  \int_{0}^{1} \lambda f(y) \,d \lambda +  \int_{0}^{1} (1 - \lambda) f(x) \,d \lambda
    \end{equation}

    \begin{equation}
        \label{eq:example}
            f(y) \int_{0}^{1} \lambda \,d \lambda +  f(x) \int_{0}^{1} (1 - \lambda) \,d \lambda
    \end{equation}

    \begin{equation}
        \label{eq:example}
            f(y) ([\frac{\lambda^2}{2}]^1_0) +  f(x) ([\lambda - \frac{\lambda^2}{2}]^1_0)
    \end{equation}

    \begin{equation}
        \label{eq:example}
            f(y) (\frac{1}{2}) +  f(x) (\frac{1}{2}) = \frac{f(x) + f(y)}{2}
    \end{equation}

We have shown that: 
    \begin{equation}
        \label{eq:example}
            \int_{0}^{1} f(x + \lambda(y - x)) \,d \lambda \leq \frac{f(x) + f(y)}{2}
    \end{equation}

Step 2: "If" Part \newline 
We know that $\int_{0}^{1} f(x + \lambda(y - x)) \,d \lambda \leq \frac{f(x) + f(y)}{2}$ and that $f$ is continuous. Our task is to prove that $f$ is convex. \newline 

Let's approach this proof by proving the contrapositive. Let's say that $f$ is NOT convex. This means that there exists a $\lambda_c \in [0, 1]$ where  $f((1 - \lambda_c)x + \lambda_c y) > \lambda_c f(y) + (1 - \lambda_c) f(x)$ \newline 

Let's define $F(\lambda) = f((1 - \lambda)x + \lambda y) - \lambda f(y) - (1 - \lambda) f(x)$. Since $f$ is continuous, we know that $F$ is continuous. 

We also know that, at $\lambda_c$, $F$ will have a positive value. Let $\lambda_b$ be the first point before $\lambda_c$ where $F$ crosses 0. Let $\lambda_d$ be the first point after $\lambda_c$ where $F$ crosses 0. \newline 

On the open interval $(\lambda_b, \lambda_d)$, $F(\lambda) > 0$ \newline 

Let $j = (1 - \lambda_b)x + \lambda_b y$ and $k = (1 - \lambda_d)x + \lambda_d y$ \newline 

$f(j) = f(k) = 0$

Hence, we can say that $\int_{0}^{1} f(j + \theta(k - j)) \,d \theta > \frac{f(j) + f(k)}{2}$

By proving the contrapositive, we have completed the proof
    \end{solution}
    
\end{problem}

\begin{problem}
    Suppose $f: \mathbb{R}^n \rightarrow \mathbb{R}$ is convex with $dom f = \mathbb{R}^n$, and bounded above on $\mathbb{R}^n$. Show that $f$ is constant

    \begin{solution}
        Let's do a proof by contradiction. We will first start with the assumption that $f$ is NOT constant. So there exist $\alpha, \beta$ on the domain of $f$ such that $f(\alpha) < f(\beta)$ \newline 

        Let $g(\theta) = f(\alpha + \theta(\beta - \alpha))$. Since $f$ is convex, $g$ is convex as well. We can clearly see that $g(0) < g(1)$ \newline 

        Based on the definition of convex functions, we know that: \newline 
        $g(1) \leq (1 - \frac{1}{\theta}) g(0) + \frac{1}{\theta} g(\theta)$. 

        This happens whenever $\theta > 1$ \newline 

        Let's rearrange the inequality: \newline 

        $\frac{1}{\theta} g(\theta) \geq g(1) - (1 - \frac{1}{\theta}) g(0)$ \newline 
        $g(\theta) \geq \theta g(1) - (\theta - 1) g(0)$ \newline 
        $g(\theta) \geq g(0) + \theta (g(1) - g(0))$ \newline 


        Based on this, as $\theta \rightarrow \infty$, we can see that $g(\theta)$ grows without bound. This contradicts the notion that $f$ is bounded above on $\mathbb{R}^n$
        
        
    \end{solution}  
\end{problem}

\begin{problem}
\textit{Minimizing a quadratic function.} Consider the problem of minimizing a quadratic function: \newline 
minimize $f(x) = \frac{1}{2} x^TPx + q^Tx + r,$ \newline 
where $P \in S^n$ (but we do not assume $P \succcurlyeq 0$)

\begin{enumerate}
    \item[(a)] Show that if P $\not\succcurlyeq$ 0, i.e., the objective function f is not convex, then the problem is unbounded below.

    \begin{solution}
        We are given that $P \not\succcurlyeq 0$. This means that $P$ is NOT positive semidefinite. \newline 

        There exists a $z$ such that $z^TPz < 0$. Now, let's plug in $\lambda z$ into our equation. 

        $f(\lambda z) = \frac{1}{2} (\lambda z)^TP(\lambda z) + q^T(\lambda z) + r$
        $f(\lambda z) = \frac{\lambda^2}{2} z^TPz + \lambda q^Tz + r$ \newline 

        As $\lambda \rightarrow \infty$, we see that $f(\lambda z) \rightarrow -\infty$. This means that the functions is UNBOUNDED below 

    \end{solution}

    \item[(b)] Now suppose that P $\succcurlyeq$ 0 (so the objective function is convex), but the optimality condition $Px^* = -q$ does not have a solution. Show that the problem is unbounded below. \newline 

    Since the optimality condition $Px^* = -q$ does not have a solution, $q$ is NOT in the column space of $P$. Hence, $q$ can be expressed as $q = q_2 + q_3$ where $q_2$ is the projection of $q$ onto the column space of $P$ and $q_3$ is orthogonal to the column space. \newline 


    Since $q_3$ is orthogonal to the column space of $P$, we can say that $q_3^TPq_3 = 0$. Let's have $\lambda q_3$. 

    $f(\lambda q_3) = \frac{1}{2} (\lambda q_3)^TP(\lambda q_3) + q^T(\lambda q_3) + r$ \newline 

    $f(\lambda q_3) = \frac{\lambda^2}{2} q_3^TPq_3 + \lambda q^Tq_3 + r$ \newline

    $f(\lambda q_3) = \lambda q^Tq_3 + r$ \newline

    $f(\lambda q_3) = \lambda (q_3 + q_2)^Tq_3 + r$ \newline

    $f(\lambda q_3) = \lambda q_3^Tq_3 + \lambda q_2^Tq_3 + r$ \newline

    $f(\lambda q_3) = \lambda q_3^Tq_3  + r$ \newline

    This is unbounded below. 
    
\end{enumerate}

\end{problem}

\begin{problem}
    \textit{Minimizing a quadratic-over-linear fractional function.} Consider the problem of minimizing the function $f: \mathbb{R}^n \rightarrow \mathbb{R}$, defined as:

    \begin{equation}
                        \label{eq:example}
                            f(x) = \frac{\|\mathbf{Ax - b}\|^2_2}{c^Tx + d}, \enspace dom f = \{x | c^Tx + d > 0\}
                    \end{equation}
We assume $rank A = n$ and $b \notin R(A)$ 

\begin{enumerate}
    \item[(a)] Show that f is closed.
    \begin{solution}
        Based on the description, it is clear to see that the domain of $f$ is open. Hence, if we prove that for every sequence $x_i \in dom f$ such that $\lim_{i} x_i = x \in bd \enspace dom f$, we have $\lim_{i\to\infty} f(x_i) = \infty$, then we can show that $f$ is closed. \newline 

        Since $b \notin R(A)$, we can see that $\|\mathbf{Ax - b}\|^2_2$ is lower bounded by a positive real number. Hence, for any given sequence $H$ where $H$ is fully contained in the domain of $f$ and the limit point of $H$ is on the boundary of the domain of $f$, we can see that as $H$ approaches its limit point, $f(x)$ will approach infinity. \newline 

        Let's further analyze this. Clearly, the boundary of the domain is when $c^Tx + d = 0$. Since $\|\mathbf{Ax - b}\|^2_2$  is lower bounded by a positive real number, we can say that $\|\mathbf{Ax - b}\|^2_2 \geq k$ where $k$ is some positive real number. So, we can rewrite our function as  $f(x) = \frac{\|\mathbf{Ax - b}\|^2_2}{c^Tx + d} \geq \frac{k}{c^Tx + d}$. Obviously, as we approach the boundary of the domain, the denominator of $\frac{k}{c^Tx + d}$ approaches 0 and $\frac{k}{c^Tx + d}$ approaches infinity. Since $f(x) = \frac{\|\mathbf{Ax - b}\|^2_2}{c^Tx + d} \geq \frac{k}{c^Tx + d}$, $f(x)$ will approach infinity as well! 
    \end{solution}
    \item[(b)] Show that the minimizer $x^*$ of $f$ is given by 
    \begin{equation}
                        \label{eq:example}
                            x^* = x_1 + tx_2
                    \end{equation}
    where $x_1 = (A^TA)^{-1} A^Tb$, $x_2 = (A^TA)^{-1}c$, and $t \in \mathbb{R}$ can be calculated by solving a quadratic equation.

    \begin{solution}
        To minimize, as we covered in the course, the first step is to take the gradient and set it to 0. \newline 

        $\nabla f = \frac{2A^T (Ax - b)(c^Tx + d)}{(c^Tx + d) ^ 2} - \frac{\|\mathbf{Ax - b}\|^2_2 (c)}{(c^Tx + d) ^ 2}$ \newline 

        $\nabla f = \frac{2A^T (Ax - b)}{(c^Tx + d)} - \frac{\|\mathbf{Ax - b}\|^2_2 (c)}{(c^Tx + d) ^ 2}$ \newline 

        $\nabla f = \frac{2A^T A (x - x_1)}{(c^Tx + d)} - \frac{\|\mathbf{Ax - b}\|^2_2 (c)}{(c^Tx + d) ^ 2}$ \newline 

        $\nabla f = \frac{2A^T A (x - x_1)}{(c^Tx + d)} - \frac{\|\mathbf{Ax - b}\|^2_2 (A^T A x_2)}{(c^Tx + d) ^ 2}$ \newline 

        $\nabla f = A^T A (\frac{2 (x - x_1)}{(c^Tx + d)} - \frac{\|\mathbf{Ax - b}\|^2_2 x_2}{(c^Tx + d) ^ 2})$ \newline 

        Now, let's set this gradient to 0 \newline 

        $\nabla f = A^T A (\frac{2 (x - x_1)}{(c^Tx + d)} - \frac{\|\mathbf{Ax - b}\|^2_2 x_2}{(c^Tx + d) ^ 2}) = 0$ \newline 

        $\nabla f = \frac{2 (x - x_1)}{(c^Tx + d)} - \frac{\|\mathbf{Ax - b}\|^2_2 x_2}{(c^Tx + d) ^ 2} = 0$ \newline 

        We know that $x - x_1 = tx_2$ \newline 

        $\nabla f = \frac{2 tx_2}{(c^Tx + d)} - \frac{\|\mathbf{Ax - b}\|^2_2 x_2}{(c^Tx + d) ^ 2} = 0$ \newline 

         $\nabla f = x_2 (\frac{2 t}{(c^Tx + d)} - \frac{\|\mathbf{Ax - b}\|^2_2 }{(c^Tx + d) ^ 2}) = 0$ \newline 

         $\nabla f = \frac{2 t}{(c^Tx + d)} - \frac{\|\mathbf{Ax - b}\|^2_2 }{(c^Tx + d) ^ 2} = 0$ \newline 

         $\frac{2 t}{(c^Tx + d)}  = \frac{\|\mathbf{Ax - b}\|^2_2 }{(c^Tx + d) ^ 2}$ \newline 

         $t = \frac{\|\mathbf{Ax - b}\|^2_2 }{2(c^Tx + d)}$ \newline 

         $t = \frac{\|\mathbf{Ax_1 + Atx_2 - b}\|^2_2 }{2(c^Tx_1 + tc^Tx_2 + d)}$ \newline 


         $2t^2 c^Tx_2 + 2t(c^Tx_1 + d) = t^2 \|\mathbf{Ax_2}\|^2_2 + 2t(Ax_1 - b)^T Ax_2 +  \|\mathbf{Ax_1 - b}\|^2_2 $ \newline 

         $2t^2 c^Tx_2 + 2t(c^Tx_1 + d) = t^2 c^T x_2 +  \|\mathbf{Ax_1 - b}\|^2_2  = 0$ \newline 

         $t^2 c^Tx_2 + 2t(c^Tx_1 + d) - \|\mathbf{Ax_1 - b}\|^2_2  = 0 $ \newline 

         The roots of this equation are: \newline 

         $t = \frac{-(c^Tx_1 + d) \pm \sqrt{(c^Tx_1 + d)^2 + c^Tx_2 \|\mathbf{Ax_1 - b}\|^2_2}}{c^Tx_2}$

        As given by the domain restriction, we just need to solve for the value of $t$ such that: \newline 

        $c^T(x) + d > 0$ \newline 
        $c^T(x_1 + tx_2) + d > 0$ \newline 

        Given the equation for the roots, we can proceed from there: \newline 

        $t = \frac{-(c^Tx_1 + d) \pm \sqrt{(c^Tx_1 + d)^2 + c^Tx_2 \|\mathbf{Ax_1 - b}\|^2_2}}{c^Tx_2}$ \newline 

        Multiply both sides by $c^Tx_2$ \newline 

        $c^Tx_2 t = -(c^Tx_1 + d) \pm \sqrt{(c^Tx_1 + d)^2 + c^Tx_2 \|\mathbf{Ax_1 - b}\|^2_2}$ \newline 

        $(c^Tx_1 + d) + c^Tx_2 t = \pm \sqrt{(c^Tx_1 + d)^2 + c^Tx_2 \|\mathbf{Ax_1 - b}\|^2_2}$ \newline 

        $c^T(x_1 + tx_2) + d = \pm \sqrt{(c^Tx_1 + d)^2 + c^Tx_2 \|\mathbf{Ax_1 - b}\|^2_2}$
        

        Since we want $c^T(x_1 + tx_2) + d > 0$ \newline 
        we can just say that we want  
        $\sqrt{(c^Tx_1 + d)^2 + c^Tx_2 \|\mathbf{Ax_1 - b}\|^2_2} > 0$

         
        
        
    \end{solution}
\end{enumerate}
\end{problem}

\end{document}





